IsarMathLib/Loop_ZF.thy
@@ -31,7 +31,7 @@ EVEN IF ADVISED OF THE POSSIBILITY OF SUCH DAMAGE.
 
 section \<open> Loops \<close>
 
-theory Loop_ZF imports Quasigroup_ZF
+theory Loop_ZF imports Quasigroup_ZF Fold_ZF
 
 begin
 
@@ -39,11 +39,11 @@ text\<open>This theory specifies the definition and proves basic  properites of 
   Loops are very similar to groups, the only property that is missing is associativity 
   of the operation.\<close>
 
-subsection\<open> Definitions and notation \<close>
+subsection\<open>Definitions and notation\<close>
 
 text\<open> In this section we define the notions of identity element and left and right inverse. \<close>
 
-text\<open> A loop is a quasigroup with an identity elemen. \<close>
+text\<open> A loop is a quasigroup with an identity element. \<close>
 
 definition "IsAloop(G,A) \<equiv> IsAquasigroup(G,A) \<and> (\<exists>e\<in>G. \<forall>x\<in>G. A`\<langle>e,x\<rangle> = x \<and> A`\<langle>x,e\<rangle> = x)"
 
@@ -65,6 +65,12 @@ locale loop0 = quasigroup0 +
 
   fixes neut ("\<one>")
   defines neut_def[simp]: "\<one> \<equiv> TheNeutralElement(G,A)"
+
+  fixes listprod ("\<Prod> _" 70)
+  defines listprod_def [simp]: "\<Prod>s \<equiv> Fold(A,\<one>,s)"
+
+  fixes pow
+  defines pow_def [simp]: "pow(n,x) \<equiv> \<Prod>{\<langle>k,x\<rangle>. k\<in>n}"
 
 text\<open> In the loop context the pair \<open>(G,A)\<close> forms a loop. \<close>
 
@@ -102,6 +108,11 @@ proof -
   ultimately show "\<one>\<in>G" and "\<forall>x\<in>G. \<one>\<cdot>x = x \<and> x\<cdot>\<one> = x"
     by auto
 qed
+
+text\<open>A loop is not empty as it contains the neutral element.\<close>
+
+corollary (in loop0) loop_not_empty: shows "G\<noteq>\<emptyset>" using neut_props_loop(1) 
+  by auto
 
 text\<open>Every element of a loop has unique left and right inverse (which need not be the same). 
   Here we define the left inverse as a function on $G$. \<close>
@@ -142,6 +153,61 @@ proof -
     by (rule ZF1_1_L9)
   with assms show "x\<cdot>(RightInv(G,A)`(x)) = \<one>" 
     using lr_inv_fun(2) ZF_fun_from_tot_val unfolding RightInv_def by simp
+qed
+
+subsection\<open>Product of a list of loop elements\<close>
+
+text\<open>Given a list $s:n\rightarrow L$ of loop elements we can define the product of the elements
+  $s=[x_0,x_1,...,x_{n-1}]$ as the fold of loop operation over that list. 
+  The \<open>loop0\<close> locale defined a notation for such fold as $\prod s$.
+  That locale also defines a notation for the special case when the list is constant i.e. 
+  $x_0 = x_1 = ... x_{n-1} = x$. In such case $\prod s$ becomes $x^{n-1}$. 
+  There are similar sections on this subject in \<open>Semigroup_ZF\<close>, \<open>Monoid_ZF\<close> and \<open>Group_ZF\<close>.
+  \<close>
+
+text\<open>The product of a list of loop elements is an element of the loop.\<close>
+
+lemma (in loop0) list_prod_in_loop: assumes "n\<in>nat" "s:n\<rightarrow>G" 
+  shows "(\<Prod>s) \<in> G"
+  using qgroupassum assms neut_props_loop(1) fold_props(2)
+  unfolding IsAquasigroup_def by force
+
+text\<open>In particular a natural power of a loop element is an element of the loop.\<close>
+
+lemma (in loop0) loop_prod_type: assumes "n\<in>nat" "x\<in>G" shows "pow(n,x) \<in> G"
+  using assms ZF_fun_from_total list_prod_in_loop by simp
+
+text\<open>For a nonempty list of loop element the last element of the list can be pulled out
+  of the product and put after the product. In other words 
+  $\prod{k=0}^n s(n) = (\prod{k=0}^{n-1} s(n))\cdot s(n)$.\<close>
+
+lemma (in loop0) loop_prod_pull_last: assumes "n \<in> nat" "\<forall>k\<in>n #+ 1. s(k) \<in> G"
+  shows "(\<Prod>{\<langle>k,s(k)\<rangle>. k\<in>n #+ 1}) = (\<Prod>{\<langle>k,s(k)\<rangle>. k\<in>n}) \<cdot> s(n)"
+  using qgroupassum assms neut_props_loop(1) fold_detach_last
+  unfolding IsAquasigroup_def by auto
+
+text\<open>The way we defined the product notation implies that the product of an empty list is the
+  neutral element of the loop. \<close>
+
+lemma (in loop0) loop_prod_empty: assumes "s:\<emptyset>\<rightarrow>G" shows "(\<Prod>s) = \<one>"
+  using qgroupassum assms neut_props_loop(1) fold_empty
+  unfolding IsAquasigroup_def by force
+
+text\<open>In particular, any loop element raised to the natural zero'th power is the 
+  neutral element of the loop. In other words $x^0=1$.\<close>
+
+corollary (in loop0) loop_zero_pow: shows "pow(0,x) = \<one>" using loop_prod_empty by simp
+  
+text\<open>Raising a loop element to a power greater by one corresponds to multiplying the power 
+  by that loop element.\<close>
+
+lemma (in loop0) loop_pow_mult_one: assumes "n\<in>nat" "x\<in>G"
+  shows "pow(n #+ 1,x) = pow(n,x)\<cdot>x"
+proof -
+  from assms(2) have "\<forall>k\<in>n #+ 1. x \<in> G" by simp
+  with assms(1) have "(\<Prod>{\<langle>k,x\<rangle>. k\<in>n #+ 1}) = (\<Prod>{\<langle>k,x\<rangle>. k\<in>n})\<cdot>x"
+    by (rule loop_prod_pull_last)
+  thus "pow(n #+ 1,x) = pow(n,x)\<cdot>x" by simp
 qed
 
 end
